hpsim with ctx, fmr

proofmode/HPSim.v
@@ -31,175 +31,185 @@ Section HPSIM.
   Variable Ist: Any.t -> Any.t -> iProp.
 
   Inductive _hpsim {with_dummy: bool}
-    (hpsim: forall R (RR: Any.t * R -> Any.t * R -> iProp), bool -> bool -> Any.t * itree hAGEs R -> Any.t * itree hAGEs R -> Σ -> Prop)
-    {R} {RR: Any.t * R -> Any.t * R -> iProp}: bool -> bool -> Any.t * itree hAGEs R -> Any.t * itree hAGEs R -> Σ -> Prop :=
+    (hpsim: forall R (RR: Any.t * R -> Any.t * R -> Σ -> iProp), bool -> bool -> Any.t * itree hAGEs R -> Any.t * itree hAGEs R -> Σ -> Σ -> Prop)
+    {R} {RR: Any.t * R -> Any.t * R -> Σ -> iProp}: bool -> bool -> Any.t * itree hAGEs R -> Any.t * itree hAGEs R -> Σ -> Σ -> Prop :=
   | hpsim_ret
       (* Note: (INV: Own fmr ⊢ #=> Ist st_src st_tgt) is required only for the funtion end. *)
       (HPSIM_RET: True)
-      ps pt st_src st_tgt fmr
+      ps pt st_src st_tgt ctx fmr
       v_src v_tgt
-      (RET: Own fmr ⊢ #=> RR (st_src,v_src) (st_tgt,v_tgt))
+      (RET: Own fmr ⊢ RR (st_src,v_src) (st_tgt,v_tgt) ctx)
     :
-    _hpsim hpsim ps pt (st_src, Ret v_src) (st_tgt, Ret v_tgt) fmr
+    _hpsim hpsim ps pt (st_src, Ret v_src) (st_tgt, Ret v_tgt) ctx fmr
+
   | hpsim_call
       (HPSIM_CALL: True)
-      ps pt st_src st_tgt fmr
+      ps pt st_src st_tgt ctx fmr fmr0
       fn varg k_src k_tgt FR
-      (INV: Own fmr ⊢ #=> (Ist st_src st_tgt ** FR))
-      (K: forall vret st_src0 st_tgt0 fmr0 
-                 (WF: URA.wf fmr0)
-                 (INV: Own fmr0 ⊢ #=> (Ist st_src0 st_tgt0 ** FR)),
-          _hpsim hpsim true true (st_src0, k_src vret) (st_tgt0, k_tgt vret) fmr0)				
+      (UPD: URA.wf (fmr0 ⋅ ctx))
+      (INV: Own fmr0 ⊢ (Ist st_src st_tgt ** FR))
+      (K: forall vret st_src0 st_tgt0 ctx' fmr' (WF: URA.wf (fmr' ⋅ ctx'))
+                 (INV: Own fmr' ⊢ (Ist st_src0 st_tgt0 ** FR)),
+          _hpsim hpsim true true (st_src0, k_src vret) (st_tgt0, k_tgt vret) ctx' fmr')
     :
-    _hpsim hpsim ps pt (st_src, trigger (Call fn varg) >>= k_src) (st_tgt, trigger (Call fn varg) >>= k_tgt) fmr
+    _hpsim hpsim ps pt (st_src, trigger (Call fn varg) >>= k_src) (st_tgt, trigger (Call fn varg) >>= k_tgt) ctx fmr
+
   | hpsim_syscall
       (HPSIM_SYSCALL: True)
-      ps pt st_src st_tgt fmr
+      ps pt st_src st_tgt ctx fmr
       fn varg rvs k_src k_tgt
       (K: forall vret, 
-          _hpsim hpsim true true (st_src, k_src vret) (st_tgt, k_tgt vret) fmr)
+          _hpsim hpsim true true (st_src, k_src vret) (st_tgt, k_tgt vret) ctx fmr)
     :
-    _hpsim hpsim ps pt (st_src, trigger (Syscall fn varg rvs) >>= k_src) (st_tgt, trigger (Syscall fn varg rvs) >>= k_tgt) fmr
+    _hpsim hpsim ps pt (st_src, trigger (Syscall fn varg rvs) >>= k_src) (st_tgt, trigger (Syscall fn varg rvs) >>= k_tgt) ctx fmr
 
   | hpsim_inline_src
       (HPSIM_INLINE_SRC: True)
-      ps pt st_src st_tgt fmr
+      ps pt st_src st_tgt ctx fmr
       fn f varg k_src i_tgt
       (FUN: alist_find fn fl_src = Some f)
-      (K: _hpsim hpsim true pt (st_src, f varg >>= (if with_dummy then (fun x => trigger (Guarantee True) ;;; trigger (Assume True) ;;; k_src x) else k_src)) (st_tgt, i_tgt) fmr)
+      (K: _hpsim hpsim true pt (st_src, f varg >>= (if with_dummy then (fun x => trigger (Guarantee True) ;;; trigger (Assume True) ;;; k_src x) else k_src)) (st_tgt, i_tgt) ctx fmr)
     :
-    _hpsim hpsim ps pt (st_src, trigger (Call fn varg) >>= k_src) (st_tgt, i_tgt) fmr
+    _hpsim hpsim ps pt (st_src, trigger (Call fn varg) >>= k_src) (st_tgt, i_tgt) ctx fmr
 
   | hpsim_inline_tgt
       (HPSIM_INLINE_TGT: True)
-      ps pt st_src st_tgt fmr
+      ps pt st_src st_tgt ctx fmr
       fn f varg i_src k_tgt
       (FUN: alist_find fn fl_tgt = Some f)
-      (K: _hpsim hpsim ps true (st_src, i_src) (st_tgt, f varg >>= (if with_dummy then (fun x => trigger (Guarantee True) ;;; trigger (Assume True) ;;; k_tgt x) else k_tgt)) fmr)
+      (K: _hpsim hpsim ps true (st_src, i_src) (st_tgt, f varg >>= (if with_dummy then (fun x => trigger (Guarantee True) ;;; trigger (Assume True) ;;; k_tgt x) else k_tgt)) ctx fmr)
     :
-    _hpsim hpsim ps pt (st_src, i_src) (st_tgt, trigger (Call fn varg) >>= k_tgt) fmr
+    _hpsim hpsim ps pt (st_src, i_src) (st_tgt, trigger (Call fn varg) >>= k_tgt) ctx fmr
 
   | hpsim_tau_src
       (HPSIM_TAU_SRC: True)
-      ps pt st_src st_tgt fmr
+      ps pt st_src st_tgt ctx fmr
       i_src i_tgt
-      (K: _hpsim hpsim true pt (st_src, i_src) (st_tgt, i_tgt) fmr)
+      (K: _hpsim hpsim true pt (st_src, i_src) (st_tgt, i_tgt) ctx fmr)
     :
-    _hpsim hpsim ps pt (st_src, tau;; i_src) (st_tgt, i_tgt) fmr
+    _hpsim hpsim ps pt (st_src, tau;; i_src) (st_tgt, i_tgt) ctx fmr
 
   | hpsim_tau_tgt
       (HPSIM_TAU_TGT: True)
-      ps pt st_src st_tgt fmr
+      ps pt st_src st_tgt ctx fmr
       i_src i_tgt
-      (K: _hpsim hpsim ps true (st_src, i_src) (st_tgt, i_tgt) fmr)
+      (K: _hpsim hpsim ps true (st_src, i_src) (st_tgt, i_tgt) ctx fmr)
     :
-    _hpsim hpsim ps pt (st_src, i_src) (st_tgt, tau;; i_tgt) fmr
-
-  | hpsim_choose_src
-      (HPSIM_CHOOSE_SRC: True)
-      ps pt st_src st_tgt fmr
-      X x k_src i_tgt
-      (K: _hpsim hpsim true pt (st_src, k_src x) (st_tgt, i_tgt) fmr)
-    :
-    _hpsim hpsim ps pt (st_src, trigger (Choose X) >>= k_src) (st_tgt, i_tgt) fmr
-
-  | hpsim_choose_tgt
-      (HPSIM_CHOOSE_TGT: True)
-      ps pt st_src st_tgt fmr
-      X i_src k_tgt
-      (K: forall (x: X), _hpsim hpsim ps true (st_src, i_src) (st_tgt, k_tgt x) fmr)
-    :
-    _hpsim hpsim ps pt (st_src, i_src) (st_tgt, trigger (Choose X) >>= k_tgt) fmr
+    _hpsim hpsim ps pt (st_src, i_src) (st_tgt, tau;; i_tgt) ctx fmr
 
   | hpsim_take_src
       (HPSIM_TAKE_SRC: True)
-      ps pt st_src st_tgt fmr
+      ps pt st_src st_tgt ctx fmr
       X k_src i_tgt
-      (K: forall (x: X), _hpsim hpsim true pt (st_src, k_src x) (st_tgt, i_tgt) fmr)
+      (K: forall (x: X), _hpsim hpsim true pt (st_src, k_src x) (st_tgt, i_tgt) ctx fmr)
     :
-    _hpsim hpsim ps pt (st_src, trigger (Take X) >>= k_src) (st_tgt, i_tgt) fmr
+    _hpsim hpsim ps pt (st_src, trigger (Take X) >>= k_src) (st_tgt, i_tgt) ctx fmr
+
+  | hpsim_choose_tgt
+      (HPSIM_CHOOSE_TGT: True)
+      ps pt st_src st_tgt ctx fmr
+      X i_src k_tgt
+      (K: forall (x: X), _hpsim hpsim ps true (st_src, i_src) (st_tgt, k_tgt x) ctx fmr)
+    :
+    _hpsim hpsim ps pt (st_src, i_src) (st_tgt, trigger (Choose X) >>= k_tgt) ctx fmr
+
+  | hpsim_choose_src
+      (HPSIM_CHOOSE_SRC: True)
+      ps pt st_src st_tgt ctx fmr
+      X x k_src i_tgt
+      (K: _hpsim hpsim true pt (st_src, k_src x) (st_tgt, i_tgt) ctx fmr)
+    :
+    _hpsim hpsim ps pt (st_src, trigger (Choose X) >>= k_src) (st_tgt, i_tgt) ctx fmr
 
   | hpsim_take_tgt
       (HPSIM_TAKE_TGT: True)
-      ps pt st_src st_tgt fmr
+      ps pt st_src st_tgt ctx fmr
       X x i_src k_tgt
-      (K: _hpsim hpsim ps true (st_src, i_src) (st_tgt, k_tgt x) fmr)
+      (K: _hpsim hpsim ps true (st_src, i_src) (st_tgt, k_tgt x) ctx fmr)
     :
-    _hpsim hpsim ps pt (st_src, i_src) (st_tgt, trigger (Take X) >>= k_tgt) fmr
+    _hpsim hpsim ps pt (st_src, i_src) (st_tgt, trigger (Take X) >>= k_tgt) ctx fmr
 
   | hpsim_supdate_src
       (HPSIM_SUPDATE_SRC: True)
-      ps pt st_src st_tgt fmr
+      ps pt st_src st_tgt ctx fmr
       X x st_src0 k_src i_tgt
       (run: Any.t -> Any.t * X)
       (RUN: run st_src = (st_src0, x))
-      (K: _hpsim hpsim true pt (st_src0, k_src x) (st_tgt, i_tgt) fmr)
+      (K: _hpsim hpsim true pt (st_src0, k_src x) (st_tgt, i_tgt) ctx fmr)
     :
-    _hpsim hpsim ps pt (st_src, trigger (SUpdate run) >>= k_src) (st_tgt, i_tgt) fmr
+    _hpsim hpsim ps pt (st_src, trigger (SUpdate run) >>= k_src) (st_tgt, i_tgt) ctx fmr
 
   | hpsim_supdate_tgt
       (HPSIM_SUPDATE_TGT: True)
-      ps pt st_src st_tgt fmr
+      ps pt st_src st_tgt ctx fmr
       X x st_tgt0 i_src k_tgt
       (run: Any.t -> Any.t * X)
       (RUN: run st_tgt = (st_tgt0, x))
-      (K: _hpsim hpsim ps true (st_src, i_src) (st_tgt0, k_tgt x) fmr)
+      (K: _hpsim hpsim ps true (st_src, i_src) (st_tgt0, k_tgt x) ctx fmr)
     :
-    _hpsim hpsim ps pt (st_src, i_src) (st_tgt, trigger (SUpdate run) >>= k_tgt) fmr
+    _hpsim hpsim ps pt (st_src, i_src) (st_tgt, trigger (SUpdate run) >>= k_tgt) ctx fmr
 
   | hpsim_assume_src
       (HPSIM_ASSUME_SRC: True)
-      ps pt st_src st_tgt fmr
-      iP k_src i_tgt FMR
-      (CUR: Own fmr ⊢ #=> FMR)
-      (K: forall fmr0 (WF: URA.wf fmr0) (NEW: Own fmr0 ⊢ #=> (iP ** FMR)),
-          _hpsim hpsim true pt (st_src, k_src tt) (st_tgt, i_tgt) fmr0)
+      ps pt st_src st_tgt ctx fmr fmr0
+      iP k_src i_tgt (FMR: iProp)
+      (UPD: URA.wf (fmr0 ⋅ ctx))
+      (CUR: Own fmr0 ⊢ FMR)
+      (K: forall ctx' fmr' (WF: URA.wf (fmr' ⋅ ctx'))
+                 (NEW: Own fmr' ⊢ (iP ** FMR)),
+          _hpsim hpsim true pt (st_src, k_src tt) (st_tgt, i_tgt) ctx' fmr')
     :
-    _hpsim hpsim ps pt (st_src, trigger (Assume iP) >>= k_src) (st_tgt, i_tgt) fmr
-
-  | hpsim_assume_tgt
-      (HPSIM_ASSUME_TGT: True)
-      ps pt st_src st_tgt fmr
-      iP i_src k_tgt FMR
-      (CUR: Own fmr ⊢ #=> (iP ** FMR))
-      (K: forall fmr0 (WF: URA.wf fmr0) (NEW: Own fmr0 ⊢ #=> FMR),
-          _hpsim hpsim ps true (st_src, i_src) (st_tgt, k_tgt tt) fmr0)
-    :
-    _hpsim hpsim ps pt (st_src, i_src) (st_tgt, trigger (Assume iP) >>= k_tgt) fmr
-
-  | hpsim_guarantee_src
-      (HPSIM_GUARANTEE_SRC: True)
-      ps pt st_src st_tgt fmr
-      iP k_src i_tgt FMR
-      (CUR: Own fmr ⊢ #=> (iP ** FMR))
-      (K: forall fmr0 (WF: URA.wf fmr0) (NEW: Own fmr0 ⊢ #=> FMR),
-          _hpsim hpsim true pt (st_src, k_src tt) (st_tgt, i_tgt) fmr0)
-    :
-    _hpsim hpsim ps pt (st_src, trigger (Guarantee iP) >>= k_src) (st_tgt, i_tgt) fmr
+    _hpsim hpsim ps pt (st_src, trigger (Assume iP) >>= k_src) (st_tgt, i_tgt) ctx fmr
 
   | hpsim_guarantee_tgt
       (HPSIM_GUARANTEE_TGT: True)
-      ps pt st_src st_tgt fmr
-      iP i_src k_tgt FMR
-      (CUR: Own fmr ⊢ #=> FMR)
-      (K: forall fmr0 (WF: URA.wf fmr0) (NEW: Own fmr0 ⊢ #=> (iP ** FMR)),
-          _hpsim hpsim ps true (st_src, i_src) (st_tgt, k_tgt tt) fmr0)
+      ps pt st_src st_tgt ctx fmr fmr0
+      iP i_src k_tgt (FMR: iProp)
+      (UPD: URA.wf (fmr0 ⋅ ctx))
+      (CUR: Own fmr0 ⊢ FMR)
+      (K: forall ctx' fmr' (WF: URA.wf (fmr' ⋅ ctx'))
+                 (NEW: Own fmr' ⊢ (iP ** FMR)),
+          _hpsim hpsim true pt (st_src, i_src) (st_tgt, k_tgt tt) ctx' fmr')
     :
-    _hpsim hpsim ps pt (st_src, i_src) (st_tgt, trigger (Guarantee iP) >>= k_tgt) fmr
+    _hpsim hpsim ps pt (st_src, i_src) (st_tgt, trigger (Guarantee iP) >>= k_tgt) ctx fmr
+
+  | hpsim_guarantee_src
+      (HPSIM_GUARANTEE_SRC: True)
+      ps pt st_src st_tgt ctx fmr fmr0
+      iP k_src i_tgt (FMR: iProp)
+      (UPD: URA.wf (fmr0 ⋅ ctx))
+      (CUR: Own fmr0 ⊢ (iP ** FMR))
+      (K: forall ctx' fmr' (WF: URA.wf (fmr' ⋅ ctx'))
+                 (NEW: Own fmr' ⊢ FMR),
+          _hpsim hpsim ps true (st_src, k_src tt) (st_tgt, i_tgt) ctx' fmr')
+    :
+    _hpsim hpsim ps pt (st_src, trigger (Guarantee iP) >>= k_src) (st_tgt, i_tgt) ctx fmr
+
+  | hpsim_assume_tgt
+      (HPSIM_ASSUME_TGT: True)
+      ps pt st_src st_tgt ctx fmr fmr0
+      iP i_src k_tgt (FMR: iProp)
+      (UPD: URA.wf (fmr0 ⋅ ctx))
+      (CUR: Own fmr0 ⊢ (iP ** FMR))
+      (K: forall ctx' fmr' (WF: URA.wf (fmr' ⋅ ctx'))
+                 (NEW: Own fmr' ⊢ FMR),
+          _hpsim hpsim ps true (st_src, i_src) (st_tgt, k_tgt tt) ctx' fmr')
+    :
+    _hpsim hpsim ps pt (st_src, i_src) (st_tgt, trigger (Assume iP) >>= k_tgt) ctx fmr
 
   | hpsim_progress
       (HPSIM_PROGRESS: True)
-      st_src st_tgt fmr
+      st_src st_tgt ctx fmr
       i_src i_tgt
-      (SIM: hpsim R RR false false (st_src, i_src) (st_tgt, i_tgt) fmr)
+      (SIM: hpsim R RR false false (st_src, i_src) (st_tgt, i_tgt) ctx fmr)
     :
-    _hpsim hpsim true true (st_src, i_src) (st_tgt, i_tgt) fmr
+    _hpsim hpsim true true (st_src, i_src) (st_tgt, i_tgt) ctx fmr
   .
   Arguments _hpsim {with_dummy} hpsim {R} RR.
 
-  Definition hpsim {R} RR := paco7 (@_hpsim false) bot7 R RR.
+  Definition hpsim {R} RR := paco8 (@_hpsim false) bot8 R RR.
 
-  Lemma _hpsim_mon with_dummy: monotone7 (@_hpsim with_dummy).
+  Lemma _hpsim_mon with_dummy: monotone8 (@_hpsim with_dummy).
   Proof. 
     ii. induction IN;
       try (econs; et; ii; exploit K; i; des; et).
@@ -208,19 +218,24 @@ Section HPSIM.
   Hint Constructors _hpsim.
   Hint Unfold hpsim.
   Hint Resolve _hpsim_mon: paco.
-  Hint Resolve cpn7_wcompat: paco.
+  Hint Resolve cpn8_wcompat: paco.
 
-  Definition hpsim_end : Any.t*Any.t -> Any.t*Any.t -> iProp :=
-    fun '(st_src, v_src) '(st_tgt, v_tgt) => Ist st_src st_tgt ** ⌜v_src = v_tgt⌝.
+  Definition hpsim_tail : Any.t*Any.t -> Any.t*Any.t -> Σ -> iProp :=
+    fun '(st_src, v_src) '(st_tgt, v_tgt) ctx =>
+      Ist st_src st_tgt ** ⌜v_src = v_tgt⌝.
 
-  Definition hpsim_body := @hpsim Any.t hpsim_end.
-  
-  Lemma _hpsim_mon_progress r R RR (ps pt ps' pt': bool) st_src st_tgt fmr
-    (SIM: @_hpsim false r R RR ps pt st_src st_tgt fmr)
+  Definition hpsim_body := @hpsim Any.t hpsim_tail.
+
+  Definition hpsim_fun (i_src: itree hAGEs Any.t) (i_tgt: itree hAGEs Any.t):  Prop :=
+    forall st_src st_tgt ctx fmr (WF: URA.wf (fmr ⋅ ctx)) (INV: Own fmr ⊢ Ist st_src st_tgt),
+    hpsim_body false false (st_src, i_src) (st_tgt, i_tgt) ctx fmr.
+
+  Lemma _hpsim_mon_progress r R RR (ps pt ps' pt': bool) st_src st_tgt ctx fmr
+    (SIM: @_hpsim false r R RR ps pt st_src st_tgt ctx fmr)
     (LES: ps -> ps')
     (LET: pt -> pt')
     :
-    @_hpsim false r R RR ps' pt' st_src st_tgt fmr.
+    @_hpsim false r R RR ps' pt' st_src st_tgt ctx fmr.
   Proof.
     move SIM before RR. revert_until SIM.
     induction SIM; i; eauto with paco.
@@ -228,16 +243,16 @@ Section HPSIM.
     destruct ps', pt'; clarify. eauto with paco.
   Qed.
 
-  Lemma hpsim_mon_progress R RR (ps pt ps' pt': bool) st_src st_tgt fmr
-    (SIM: @hpsim R RR ps pt st_src st_tgt fmr)
+  Lemma hpsim_mon_progress R RR (ps pt ps' pt': bool) st_src st_tgt ctx fmr
+    (SIM: @hpsim R RR ps pt st_src st_tgt ctx fmr)
     (LES: ps -> ps')
     (LET: pt -> pt')
     :
-    hpsim RR ps' pt' st_src st_tgt fmr.
+    hpsim RR ps' pt' st_src st_tgt ctx fmr.
   Proof.
     move SIM before RR. revert_until SIM. pcofix CIH. i.
     pstep. eapply _hpsim_mon_progress; eauto.
-    eapply paco7_mon_bot in SIM; eauto. punfold SIM.
+    eapply paco8_mon_bot in SIM; eauto. punfold SIM.
   Qed.
 
   Lemma case_itrH R (itrH: itree hAGEs R) :
@@ -264,60 +279,64 @@ Section HPSIM.
       repeat f_equal. extensionality x. rewrite bind_ret_l. eauto.
   Qed.  
 
-  Lemma hpsim_progress_flag with_dummy R RR r g st_src st_tgt fmr
-        (SIM: gpaco7 (@_hpsim with_dummy) (cpn7 (@_hpsim with_dummy)) g g R RR false false st_src st_tgt fmr)
+  Lemma hpsim_progress_flag with_dummy R RR r g st_src st_tgt ctx fmr
+        (SIM: gpaco8 (@_hpsim with_dummy) (cpn8 (@_hpsim with_dummy)) g g R RR false false st_src st_tgt ctx fmr)
       :
-        gpaco7 (@_hpsim with_dummy) (cpn7 (@_hpsim with_dummy)) r g R RR true true st_src st_tgt fmr.
+        gpaco8 (@_hpsim with_dummy) (cpn8 (@_hpsim with_dummy)) r g R RR true true st_src st_tgt ctx fmr.
   Proof.
     gstep. destruct st_src, st_tgt. econs; et.
   Qed.
 
-  Lemma hpsim_flag_mon with_dummy
-        (hpsim: forall (R: Type) (RR: Any.t * R -> Any.t * R -> iProp),  bool -> bool -> Any.t * itree hAGEs R -> Any.t * itree hAGEs R -> Σ -> Prop)
-        R (RR: Any.t * R -> Any.t * R -> iProp)
-        ps0 pt0 ps1 pt1 st_src st_tgt fmr
-        (SIM: (@_hpsim with_dummy) hpsim _ RR ps0 pt0 st_src st_tgt fmr)
+  Lemma hpsim_flag_mon with_dummy hpsim R RR
+        ps0 pt0 ps1 pt1 st_src st_tgt ctx fmr
+        (SIM: (@_hpsim with_dummy) hpsim R RR ps0 pt0 st_src st_tgt ctx fmr)
         (SRC: ps0 = true -> ps1 = true)
         (TGT: pt0 = true -> pt1 = true)
     :
-        (@_hpsim with_dummy) hpsim _ RR ps1 pt1 st_src st_tgt fmr.
+        (@_hpsim with_dummy) hpsim _ RR ps1 pt1 st_src st_tgt ctx fmr.
   Proof.
     revert ps1 pt1 SRC TGT.
     induction SIM; i; clarify; et.
     exploit SRC; et. exploit TGT; et. i. clarify. econs; et.
-  Qed.              
+  Qed.
+
+
+
+
+
+
 
   Variant hpsim_flagC 
-    (r: forall (R: Type) (RR: Any.t * R -> Any.t * R -> iProp),  bool -> bool -> Any.t * itree hAGEs R -> Any.t * itree hAGEs R -> Σ -> Prop)
-    {R} (RR: Any.t * R -> Any.t * R -> iProp): bool -> bool -> Any.t * itree hAGEs R -> Any.t * itree hAGEs R -> Σ -> Prop := 
+    (r: forall (R: Type) (RR: Any.t * R -> Any.t * R -> Σ -> iProp),  bool -> bool -> Any.t * itree hAGEs R -> Any.t * itree hAGEs R -> Σ -> Σ -> Prop)
+    R RR ps1 pt1 st_src st_tgt ctx fmr : Prop :=
   | hpsim_flagC_intro
-    ps0 pt0 ps1 pt1 st_src st_tgt fmr
-    (SIM: r _ RR ps0 pt0 st_src st_tgt fmr)
+    ps0 pt0
+    (SIM: r R RR ps0 pt0 st_src st_tgt ctx fmr)
     (SRC: ps0 = true -> ps1 = true)
     (TGT: pt0 = true -> pt1 = true)
-  :
-    hpsim_flagC r RR ps1 pt1 st_src st_tgt fmr
-  .   
+  .
 
-  Lemma hpsim_flagC_mon r1 r2 (LE: r1 <7= r2) : @hpsim_flagC r1 <7= @hpsim_flagC r2.
+  Lemma hpsim_flagC_mon r1 r2 (LE: r1 <8= r2) :
+    @hpsim_flagC r1 <8= @hpsim_flagC r2.
   Proof. ii. destruct PR; econs; et. Qed.
 
   Hint Resolve hpsim_flagC_mon: paco.
   
-  Lemma hpsim_flagC_spec with_dummy: hpsim_flagC <8= gupaco7 (@_hpsim with_dummy) (cpn7 (@_hpsim with_dummy)).
+  Lemma hpsim_flagC_spec with_dummy:
+    hpsim_flagC <9= gupaco8 (@_hpsim with_dummy) (cpn8 (@_hpsim with_dummy)).
   Proof.
-    eapply wrespect7_uclo; eauto with paco.
+    eapply wrespect8_uclo; eauto with paco.
     econs; eauto with paco. i. inv PR.
     eapply GF in SIM.
     revert x2 x3 SRC TGT. induction SIM; i; clarify; et.
     exploit SRC; et. exploit TGT; et. i. clarify. econs; et.
-    eapply rclo7_base; et.
+    eapply rclo8_base; et.
   Qed.
 
-  Lemma hpsim_flag_down with_dummy R RR r g ps pt st_src st_tgt fmr
-        (SIM: gpaco7 (@_hpsim with_dummy) (cpn7 (@_hpsim with_dummy)) r g R RR false false st_src st_tgt fmr)
+  Lemma hpsim_flag_down with_dummy R RR r g ps pt st_src st_tgt ctx fmr
+        (SIM: gpaco8 (@_hpsim with_dummy) (cpn8 (@_hpsim with_dummy)) r g R RR false false st_src st_tgt ctx fmr)
       :
-        gpaco7 (@_hpsim with_dummy) (cpn7 (@_hpsim with_dummy)) r g R RR ps pt st_src st_tgt fmr.
+        gpaco8 (@_hpsim with_dummy) (cpn8 (@_hpsim with_dummy)) r g R RR ps pt st_src st_tgt ctx fmr.
   Proof. 
     guclo hpsim_flagC_spec. econs; et. 
   Qed.
@@ -326,169 +345,177 @@ Section HPSIM.
 
 
 
-
   Variant hpsimC {with_dummy: bool}
-  (hpsim: forall R (RR: Any.t * R -> Any.t * R -> iProp), bool -> bool -> Any.t * itree hAGEs R -> Any.t * itree hAGEs R -> Σ -> Prop)
-  {R} {RR: Any.t * R -> Any.t * R -> iProp}: bool -> bool -> Any.t * itree hAGEs R -> Any.t * itree hAGEs R -> Σ -> Prop :=
+    (hpsim: forall R (RR: Any.t * R -> Any.t * R -> Σ -> iProp), bool -> bool -> Any.t * itree hAGEs R -> Any.t * itree hAGEs R -> Σ -> Σ -> Prop)
+    {R} {RR: Any.t * R -> Any.t * R -> Σ -> iProp}: bool -> bool -> Any.t * itree hAGEs R -> Any.t * itree hAGEs R -> Σ -> Σ -> Prop :=
   | hpsimC_ret
       (* Note: (INV: Own fmr ⊢ #=> Ist st_src st_tgt) is required only for the funtion end. *)
-      ps pt st_src st_tgt fmr
+      ps pt st_src st_tgt ctx fmr
       v_src v_tgt
-      (RET: Own fmr ⊢ #=> RR (st_src,v_src) (st_tgt,v_tgt))
+      (RET: Own fmr ⊢ RR (st_src,v_src) (st_tgt,v_tgt) ctx)
     :
-    hpsimC hpsim ps pt (st_src, Ret v_src) (st_tgt, Ret v_tgt) fmr
+    hpsimC hpsim ps pt (st_src, Ret v_src) (st_tgt, Ret v_tgt) ctx fmr
+          
   | hpsimC_call
-      ps pt st_src st_tgt fmr
+      ps pt st_src st_tgt ctx fmr fmr0
       fn varg k_src k_tgt FR
-      (INV: Own fmr ⊢ #=> (Ist st_src st_tgt ** FR))
-      (K: forall vret st_src0 st_tgt0 fmr0 
-                 (WF: URA.wf fmr0)
-                 (INV: Own fmr0 ⊢ #=> (Ist st_src0 st_tgt0 ** FR)),
-          hpsim _ RR true true (st_src0, k_src vret) (st_tgt0, k_tgt vret) fmr0)				
+      (UPD: URA.wf (fmr0 ⋅ ctx))
+      (INV: Own fmr0 ⊢ (Ist st_src st_tgt ** FR))
+      (K: forall vret st_src0 st_tgt0 ctx' fmr' (WF: URA.wf (fmr' ⋅ ctx'))
+                 (INV: Own fmr' ⊢ (Ist st_src0 st_tgt0 ** FR)),
+          hpsim R RR true true (st_src0, k_src vret) (st_tgt0, k_tgt vret) ctx' fmr')
     :
-    hpsimC hpsim ps pt (st_src, trigger (Call fn varg) >>= k_src) (st_tgt, trigger (Call fn varg) >>= k_tgt) fmr
+    hpsimC hpsim ps pt (st_src, trigger (Call fn varg) >>= k_src) (st_tgt, trigger (Call fn varg) >>= k_tgt) ctx fmr
+
   | hpsimC_syscall
-      ps pt st_src st_tgt fmr
+      ps pt st_src st_tgt ctx fmr
       fn varg rvs k_src k_tgt
       (K: forall vret, 
-          hpsim _ RR true true (st_src, k_src vret) (st_tgt, k_tgt vret) fmr)
+          hpsim R RR true true (st_src, k_src vret) (st_tgt, k_tgt vret) ctx fmr)
     :
-    hpsimC hpsim ps pt (st_src, trigger (Syscall fn varg rvs) >>= k_src) (st_tgt, trigger (Syscall fn varg rvs) >>= k_tgt) fmr
+    hpsimC hpsim ps pt (st_src, trigger (Syscall fn varg rvs) >>= k_src) (st_tgt, trigger (Syscall fn varg rvs) >>= k_tgt) ctx fmr
 
   | hpsimC_inline_src
-      ps pt st_src st_tgt fmr
+      ps pt st_src st_tgt ctx fmr
       fn f varg k_src i_tgt
       (FUN: alist_find fn fl_src = Some f)
-      (K: hpsim _ RR true pt (st_src, f varg >>= (if with_dummy then (fun x => trigger (Guarantee True) ;;; trigger (Assume True) ;;; k_src x) else k_src)) (st_tgt, i_tgt) fmr)
+      (K: hpsim R RR true pt (st_src, f varg >>= (if with_dummy then (fun x => trigger (Guarantee True) ;;; trigger (Assume True) ;;; k_src x) else k_src)) (st_tgt, i_tgt) ctx fmr)
     :
-    hpsimC hpsim ps pt (st_src, trigger (Call fn varg) >>= k_src) (st_tgt, i_tgt) fmr
+    hpsimC hpsim ps pt (st_src, trigger (Call fn varg) >>= k_src) (st_tgt, i_tgt) ctx fmr
 
   | hpsimC_inline_tgt
-      ps pt st_src st_tgt fmr
+      ps pt st_src st_tgt ctx fmr
       fn f varg i_src k_tgt
       (FUN: alist_find fn fl_tgt = Some f)
-      (K: hpsim _ RR ps true (st_src, i_src) (st_tgt, f varg >>= (if with_dummy then (fun x => trigger (Guarantee True) ;;; trigger (Assume True) ;;; k_tgt x) else k_tgt)) fmr)
+      (K: hpsim R RR ps true (st_src, i_src) (st_tgt, f varg >>= (if with_dummy then (fun x => trigger (Guarantee True) ;;; trigger (Assume True) ;;; k_tgt x) else k_tgt)) ctx fmr)
     :
-    hpsimC hpsim ps pt (st_src, i_src) (st_tgt, trigger (Call fn varg) >>= k_tgt) fmr
+    hpsimC hpsim ps pt (st_src, i_src) (st_tgt, trigger (Call fn varg) >>= k_tgt) ctx fmr
 
   | hpsimC_tau_src
-      ps pt st_src st_tgt fmr
+      ps pt st_src st_tgt ctx fmr
       i_src i_tgt
-      (K: hpsim _ RR true pt (st_src, i_src) (st_tgt, i_tgt) fmr)
+      (K: hpsim R RR true pt (st_src, i_src) (st_tgt, i_tgt) ctx fmr)
     :
-    hpsimC hpsim ps pt (st_src, tau;; i_src) (st_tgt, i_tgt) fmr
+    hpsimC hpsim ps pt (st_src, tau;; i_src) (st_tgt, i_tgt) ctx fmr
 
   | hpsimC_tau_tgt
-      ps pt st_src st_tgt fmr
+      ps pt st_src st_tgt ctx fmr
       i_src i_tgt
-      (K: hpsim _ RR ps true (st_src, i_src) (st_tgt, i_tgt) fmr)
+      (K: hpsim R RR ps true (st_src, i_src) (st_tgt, i_tgt) ctx fmr)
     :
-    hpsimC hpsim ps pt (st_src, i_src) (st_tgt, tau;; i_tgt) fmr
-
-  | hpsimC_choose_src
-      ps pt st_src st_tgt fmr
-      X x k_src i_tgt
-      (K: hpsim _ RR true pt (st_src, k_src x) (st_tgt, i_tgt) fmr)
-    :
-    hpsimC hpsim ps pt (st_src, trigger (Choose X) >>= k_src) (st_tgt, i_tgt) fmr
-
-  | hpsimC_choose_tgt
-      ps pt st_src st_tgt fmr
-      X i_src k_tgt
-      (K: forall (x: X), hpsim _ RR ps true (st_src, i_src) (st_tgt, k_tgt x) fmr)
-    :
-    hpsimC hpsim ps pt (st_src, i_src) (st_tgt, trigger (Choose X) >>= k_tgt) fmr
+    hpsimC hpsim ps pt (st_src, i_src) (st_tgt, tau;; i_tgt) ctx fmr
 
   | hpsimC_take_src
-      ps pt st_src st_tgt fmr
+      ps pt st_src st_tgt ctx fmr
       X k_src i_tgt
-      (K: forall (x: X), hpsim _ RR true pt (st_src, k_src x) (st_tgt, i_tgt) fmr)
+      (K: forall (x: X), hpsim R RR true pt (st_src, k_src x) (st_tgt, i_tgt) ctx fmr)
     :
-    hpsimC hpsim ps pt (st_src, trigger (Take X) >>= k_src) (st_tgt, i_tgt) fmr
+    hpsimC hpsim ps pt (st_src, trigger (Take X) >>= k_src) (st_tgt, i_tgt) ctx fmr
+
+  | hpsimC_choose_tgt
+      ps pt st_src st_tgt ctx fmr
+      X i_src k_tgt
+      (K: forall (x: X), hpsim R RR ps true (st_src, i_src) (st_tgt, k_tgt x) ctx fmr)
+    :
+    hpsimC hpsim ps pt (st_src, i_src) (st_tgt, trigger (Choose X) >>= k_tgt) ctx fmr
+
+  | hpsimC_choose_src
+      ps pt st_src st_tgt ctx fmr
+      X x k_src i_tgt
+      (K: hpsim R RR true pt (st_src, k_src x) (st_tgt, i_tgt) ctx fmr)
+    :
+    hpsimC hpsim ps pt (st_src, trigger (Choose X) >>= k_src) (st_tgt, i_tgt) ctx fmr
 
   | hpsimC_take_tgt
-      ps pt st_src st_tgt fmr
+      ps pt st_src st_tgt ctx fmr
       X x i_src k_tgt
-      (K: hpsim _ RR ps true (st_src, i_src) (st_tgt, k_tgt x) fmr)
+      (K: hpsim R RR ps true (st_src, i_src) (st_tgt, k_tgt x) ctx fmr)
     :
-    hpsimC hpsim ps pt (st_src, i_src) (st_tgt, trigger (Take X) >>= k_tgt) fmr
+    hpsimC hpsim ps pt (st_src, i_src) (st_tgt, trigger (Take X) >>= k_tgt) ctx fmr
 
   | hpsimC_supdate_src
-      ps pt st_src st_tgt fmr
+      ps pt st_src st_tgt ctx fmr
       X x st_src0 k_src i_tgt
       (run: Any.t -> Any.t * X)
       (RUN: run st_src = (st_src0, x))
-      (K: hpsim _ RR true pt (st_src0, k_src x) (st_tgt, i_tgt) fmr)
+      (K: hpsim R RR true pt (st_src0, k_src x) (st_tgt, i_tgt) ctx fmr)
     :
-    hpsimC hpsim ps pt (st_src, trigger (SUpdate run) >>= k_src) (st_tgt, i_tgt) fmr
+    hpsimC hpsim ps pt (st_src, trigger (SUpdate run) >>= k_src) (st_tgt, i_tgt) ctx fmr
 
   | hpsimC_supdate_tgt
-      ps pt st_src st_tgt fmr
+      ps pt st_src st_tgt ctx fmr
       X x st_tgt0 i_src k_tgt
       (run: Any.t -> Any.t * X)
       (RUN: run st_tgt = (st_tgt0, x))
-      (K: hpsim _ RR ps true (st_src, i_src) (st_tgt0, k_tgt x) fmr)
+      (K: hpsim R RR ps true (st_src, i_src) (st_tgt0, k_tgt x) ctx fmr)
     :
-    hpsimC hpsim ps pt (st_src, i_src) (st_tgt, trigger (SUpdate run) >>= k_tgt) fmr
+    hpsimC hpsim ps pt (st_src, i_src) (st_tgt, trigger (SUpdate run) >>= k_tgt) ctx fmr
 
   | hpsimC_assume_src
-      ps pt st_src st_tgt fmr
-      iP k_src i_tgt FMR
-      (CUR: Own fmr ⊢ #=> FMR)
-      (K: forall fmr0 (WF: URA.wf fmr0) (NEW: Own fmr0 ⊢ #=> (iP ** FMR)),
-          hpsim _ RR true pt (st_src, k_src tt) (st_tgt, i_tgt) fmr0)
+      ps pt st_src st_tgt ctx fmr fmr0
+      iP k_src i_tgt (FMR: iProp)
+      (UPD: URA.wf (fmr0 ⋅ ctx))
+      (CUR: Own fmr0 ⊢ FMR)
+      (K: forall ctx' fmr' (WF: URA.wf (fmr' ⋅ ctx'))
+                 (NEW: Own fmr' ⊢ (iP ** FMR)),
+          hpsim R RR true pt (st_src, k_src tt) (st_tgt, i_tgt) ctx' fmr')
     :
-    hpsimC hpsim ps pt (st_src, trigger (Assume iP) >>= k_src) (st_tgt, i_tgt) fmr
-
-  | hpsimC_assume_tgt
-      ps pt st_src st_tgt fmr
-      iP i_src k_tgt FMR
-      (CUR: Own fmr ⊢ #=> (iP ** FMR))
-      (K: forall fmr0 (WF: URA.wf fmr0) (NEW: Own fmr0 ⊢ #=> FMR),
-          hpsim _ RR ps true (st_src, i_src) (st_tgt, k_tgt tt) fmr0)
-    :
-    hpsimC hpsim ps pt (st_src, i_src) (st_tgt, trigger (Assume iP) >>= k_tgt) fmr
-
-  | hpsimC_guarantee_src
-      ps pt st_src st_tgt fmr
-      iP k_src i_tgt FMR
-      (CUR: Own fmr ⊢ #=> (iP ** FMR))
-      (K: forall fmr0 (WF: URA.wf fmr0) (NEW: Own fmr0 ⊢ #=> FMR),
-          hpsim _ RR true pt (st_src, k_src tt) (st_tgt, i_tgt) fmr0)
-    :
-    hpsimC hpsim ps pt (st_src, trigger (Guarantee iP) >>= k_src) (st_tgt, i_tgt) fmr
+    hpsimC hpsim ps pt (st_src, trigger (Assume iP) >>= k_src) (st_tgt, i_tgt) ctx fmr
 
   | hpsimC_guarantee_tgt
-      ps pt st_src st_tgt fmr
-      iP i_src k_tgt FMR
-      (CUR: Own fmr ⊢ #=> FMR)
-      (K: forall fmr0 (WF: URA.wf fmr0) (NEW: Own fmr0 ⊢ #=> (iP ** FMR)),
-          hpsim _ RR ps true (st_src, i_src) (st_tgt, k_tgt tt) fmr0)
+      ps pt st_src st_tgt ctx fmr fmr0
+      iP i_src k_tgt (FMR: iProp)
+      (UPD: URA.wf (fmr0 ⋅ ctx))
+      (CUR: Own fmr0 ⊢ FMR)
+      (K: forall ctx' fmr' (WF: URA.wf (fmr' ⋅ ctx'))
+                 (NEW: Own fmr' ⊢ (iP ** FMR)),
+          hpsim R RR true pt (st_src, i_src) (st_tgt, k_tgt tt) ctx' fmr')
     :
-    hpsimC hpsim ps pt (st_src, i_src) (st_tgt, trigger (Guarantee iP) >>= k_tgt) fmr
+    hpsimC hpsim ps pt (st_src, i_src) (st_tgt, trigger (Guarantee iP) >>= k_tgt) ctx fmr
+           
+  | hpsimC_guarantee_src
+      ps pt st_src st_tgt ctx fmr fmr0
+      iP k_src i_tgt (FMR: iProp)
+      (UPD: URA.wf (fmr0 ⋅ ctx))
+      (CUR: Own fmr0 ⊢ (iP ** FMR))
+      (K: forall ctx' fmr' (WF: URA.wf (fmr' ⋅ ctx'))
+                 (NEW: Own fmr' ⊢ FMR),
+          hpsim R RR ps true (st_src, k_src tt) (st_tgt, i_tgt) ctx' fmr')
+    :
+    hpsimC hpsim ps pt (st_src, trigger (Guarantee iP) >>= k_src) (st_tgt, i_tgt) ctx fmr
 
-  | hpsimC_progress
-      st_src st_tgt fmr
-      i_src i_tgt
-      (SIM: hpsim R RR false false (st_src, i_src) (st_tgt, i_tgt) fmr)
+  | hpsimC_assume_tgt
+      ps pt st_src st_tgt ctx fmr fmr0
+      iP i_src k_tgt (FMR: iProp)
+      (UPD: URA.wf (fmr0 ⋅ ctx))
+      (CUR: Own fmr0 ⊢ (iP ** FMR))
+      (K: forall ctx' fmr' (WF: URA.wf (fmr' ⋅ ctx'))
+                 (NEW: Own fmr' ⊢ FMR),
+          hpsim R RR ps true (st_src, i_src) (st_tgt, k_tgt tt) ctx' fmr')
     :
-    hpsimC hpsim true true (st_src, i_src) (st_tgt, i_tgt) fmr
+    hpsimC hpsim ps pt (st_src, i_src) (st_tgt, trigger (Assume iP) >>= k_tgt) ctx fmr
+           
+  | hpsimC_progress
+      st_src st_tgt ctx fmr
+      i_src i_tgt
+      (SIM: hpsim R RR false false (st_src, i_src) (st_tgt, i_tgt) ctx fmr)
+    :
+    hpsimC hpsim true true (st_src, i_src) (st_tgt, i_tgt) ctx fmr
   .
-  Arguments _hpsim {with_dummy} hpsim {R} RR.
-                
+  Arguments hpsimC {with_dummy} hpsim {R} RR.
   Hint Constructors hpsimC: paco.
   
-  Lemma hpsimC_mon with_dummy : monotone7 (@hpsimC with_dummy).
+  Lemma hpsimC_mon with_dummy : monotone8 (@hpsimC with_dummy).
   Proof.
-    ii. inv IN; try (by des; econs; ss; et).
+    ii. inv IN; try (by des; econs; et).
   Qed.
 
   Lemma hpsimC_spec with_dummy:
-    (@hpsimC with_dummy) <8= gupaco7 (@_hpsim with_dummy) (cpn7 (@_hpsim with_dummy)).
+    (@hpsimC with_dummy) <9= gupaco8 (@_hpsim with_dummy) (cpn8 (@_hpsim with_dummy)).
   Proof.
-    eapply wrespect7_uclo; eauto with paco.
+    eapply wrespect8_uclo; eauto with paco.
     econs; eauto using hpsimC_mon; i.
-    inv PR; econs; et; try (i; eapply _hpsim_mon; eauto using rclo7).
+    inv PR; econs; et; try (i; eapply _hpsim_mon; eauto using rclo8).
     econs; eauto.
   Qed.
   
@@ -497,33 +524,142 @@ Section HPSIM.
 
 
 
+  Variant safe_hpsim
+    (hpsim: forall R (RR: Any.t * R -> Any.t * R -> Σ ->iProp), bool -> bool -> Any.t * itree hAGEs R -> Any.t * itree hAGEs R -> Σ -> Σ -> Prop)
+    {R} {RR: Any.t * R -> Any.t * R -> Σ ->iProp}: bool -> bool -> Any.t * itree hAGEs R -> Any.t * itree hAGEs R -> Σ -> Σ ->Prop := 
+    | safe_hpsim_ret
+      (* Note: (INV: Own fmr ⊢ #=> Ist st_src st_tgt) is required only for the funtion end. *)
+      ps pt st_src st_tgt ctx fmr
+      v_src v_tgt
+      (RET: Own fmr ⊢ RR (st_src,v_src) (st_tgt,v_tgt) ctx)
+    :
+    safe_hpsim hpsim ps pt (st_src, Ret v_src) (st_tgt, Ret v_tgt) ctx fmr
+               
+    | safe_hpsim_call
+      ps pt st_src st_tgt ctx fmr fmr0
+      fn varg k_src k_tgt FR
+      (UPD: URA.wf (fmr0 ⋅ ctx))
+      (INV: Own fmr0 ⊢ (Ist st_src st_tgt ** FR))
+      (K: forall vret st_src0 st_tgt0 ctx' fmr' (WF: URA.wf (fmr' ⋅ ctx'))
+                 (INV: Own fmr' ⊢ (Ist st_src0 st_tgt0 ** FR)),
+          hpsim R RR true true (st_src0, k_src vret) (st_tgt0, k_tgt vret) ctx' fmr')
+    :
+    safe_hpsim hpsim ps pt (st_src, trigger (Call fn varg) >>= k_src) (st_tgt, trigger (Call fn varg) >>= k_tgt) ctx fmr
+               
+    | safe_hpsim_syscall
+      ps pt st_src st_tgt ctx fmr
+      fn varg rvs k_src k_tgt
+      (K: forall vret, 
+          hpsim R RR true true (st_src, k_src vret) (st_tgt, k_tgt vret) ctx fmr)
+    :
+    safe_hpsim hpsim ps pt (st_src, trigger (Syscall fn varg rvs) >>= k_src) (st_tgt, trigger (Syscall fn varg rvs) >>= k_tgt) ctx fmr
+
+    | safe_hpsim_tau_src
+      ps pt st_src st_tgt ctx fmr
+      i_src i_tgt
+      (K: hpsim R RR true pt (st_src, i_src) (st_tgt, i_tgt) ctx fmr)
+    :
+    safe_hpsim hpsim ps pt (st_src, tau;; i_src) (st_tgt, i_tgt) ctx fmr
+
+    | safe_hpsim_tau_tgt
+      ps pt st_src st_tgt ctx fmr
+      i_src i_tgt
+      (K: hpsim R RR ps true (st_src, i_src) (st_tgt, i_tgt) ctx fmr)
+    :
+    safe_hpsim hpsim ps pt (st_src, i_src) (st_tgt, tau;; i_tgt) ctx fmr
+
+    | safe_hpsim_take_src
+      ps pt st_src st_tgt ctx fmr
+      X k_src i_tgt
+      (K: forall (x: X), hpsim R RR true pt (st_src, k_src x) (st_tgt, i_tgt) ctx fmr)
+    :
+    safe_hpsim hpsim ps pt (st_src, trigger (Take X) >>= k_src) (st_tgt, i_tgt) ctx fmr
+
+    | safe_hpsim_choose_tgt
+      ps pt st_src st_tgt ctx fmr
+      X i_src k_tgt
+      (K: forall (x: X), hpsim R RR ps true (st_src, i_src) (st_tgt, k_tgt x) ctx fmr)
+    :
+    safe_hpsim hpsim ps pt (st_src, i_src) (st_tgt, trigger (Choose X) >>= k_tgt) ctx fmr
+
+    | safe_hpsim_supdate_src
+      ps pt st_src st_tgt ctx fmr
+      X x st_src0 k_src i_tgt
+      (run: Any.t -> Any.t * X)
+      (RUN: run st_src = (st_src0, x))
+      (K: hpsim R RR true pt (st_src0, k_src x) (st_tgt, i_tgt) ctx fmr)
+    :
+    safe_hpsim hpsim ps pt (st_src, trigger (SUpdate run) >>= k_src) (st_tgt, i_tgt) ctx fmr
+
+    | safe_hpsim_supdate_tgt
+      ps pt st_src st_tgt ctx fmr
+      X x st_tgt0 i_src k_tgt
+      (run: Any.t -> Any.t * X)
+      (RUN: run st_tgt = (st_tgt0, x))
+      (K: hpsim R RR ps true (st_src, i_src) (st_tgt0, k_tgt x) ctx fmr)
+    :
+    safe_hpsim hpsim ps pt (st_src, i_src) (st_tgt, trigger (SUpdate run) >>= k_tgt) ctx fmr
+
+    | safe_hpsim_assume_src
+      ps pt st_src st_tgt ctx fmr fmr0
+      iP k_src i_tgt (FMR: iProp)
+      (UPD: URA.wf (fmr0 ⋅ ctx))
+      (CUR: Own fmr0 ⊢ FMR)
+      (K: forall ctx' fmr' (WF: URA.wf (fmr' ⋅ ctx'))
+                 (NEW: Own fmr' ⊢ (iP ** FMR)),
+          hpsim R RR true pt (st_src, k_src tt) (st_tgt, i_tgt) ctx' fmr')
+    :
+    safe_hpsim hpsim ps pt (st_src, trigger (Assume iP) >>= k_src) (st_tgt, i_tgt) ctx fmr
+
+    | safe_hpsim_guarantee_tgt
+      ps pt st_src st_tgt ctx fmr fmr0
+      iP i_src k_tgt (FMR: iProp)
+      (UPD: URA.wf (fmr0 ⋅ ctx))
+      (CUR: Own fmr0 ⊢ FMR)
+      (K: forall ctx' fmr' (WF: URA.wf (fmr' ⋅ ctx'))
+                 (NEW: Own fmr' ⊢ (iP ** FMR)),
+          hpsim R RR true pt (st_src, i_src) (st_tgt, k_tgt tt) ctx' fmr')
+    :
+    safe_hpsim hpsim ps pt (st_src, i_src) (st_tgt, trigger (Guarantee iP) >>= k_tgt) ctx fmr
+  .
+
+  Lemma safe_hpsim_spec:
+    safe_hpsim <9= gupaco8 (@_hpsim false) (cpn8 (@_hpsim false)).
+  Proof.
+    i. eapply hpsimC_spec. depdes PR; try by (econs; et).
+  Qed.
 
 
-  Variant hpsim_bindC (r: forall R (RR: Any.t * R -> Any.t * R -> iProp), bool -> bool -> Any.t * itree hAGEs R -> Any.t * itree hAGEs R -> Σ -> Prop):
-    forall R (RR: Any.t * R -> Any.t * R -> iProp), bool -> bool -> Any.t * itree hAGEs R -> Any.t * itree hAGEs R -> Σ -> Prop
+
+
+
+  
+
+  Variant hpsim_bindC (r: forall R (RR: Any.t * R -> Any.t * R -> Σ -> iProp), bool -> bool -> Any.t * itree hAGEs R -> Any.t * itree hAGEs R -> Σ -> Σ -> Prop):
+    forall R (RR: Any.t * R -> Any.t * R -> Σ -> iProp), bool -> bool -> Any.t * itree hAGEs R -> Any.t * itree hAGEs R -> Σ -> Σ -> Prop
   :=
   | hpsim_bindC_intro
-      ps pt Q QQ st_src st_tgt i_src i_tgt fmr
-      (SIM: r Q QQ ps pt (st_src, i_src) (st_tgt, i_tgt) fmr)
+      ps pt Q QQ st_src st_tgt i_src i_tgt ctx fmr
+      (SIM: r Q QQ ps pt (st_src, i_src) (st_tgt, i_tgt) ctx fmr)
 
       R RR k_src k_tgt
-      (SIMK: forall st_src0 st_tgt0 vret_src vret_tgt fmr0
-               (RET: Own fmr0 ⊢ #=> QQ (st_src0, vret_src) (st_tgt0, vret_tgt)),
-             r R RR false false (st_src0, k_src vret_src) (st_tgt0, k_tgt vret_tgt) fmr0)
+      (SIMK: forall st_src0 st_tgt0 vret_src vret_tgt ctx' fmr'
+               (RET: Own fmr' ⊢ QQ (st_src0, vret_src) (st_tgt0, vret_tgt) ctx'),
+             r R RR false false (st_src0, k_src vret_src) (st_tgt0, k_tgt vret_tgt) ctx' fmr')
     :
-    hpsim_bindC r R RR ps pt (st_src, i_src >>= k_src) (st_tgt, i_tgt >>= k_tgt) fmr
+    hpsim_bindC r R RR ps pt (st_src, i_src >>= k_src) (st_tgt, i_tgt >>= k_tgt) ctx fmr
   .
 
   Lemma hpsim_bindC_mon
         r1 r2
-        (LEr: r1 <7= r2)
+        (LEr: r1 <8= r2)
     :
-    hpsim_bindC r1 <7= hpsim_bindC r2
+    hpsim_bindC r1 <8= hpsim_bindC r2
   .
   Proof. ii. destruct PR; econs; et. Qed.
 
   Lemma hpsim_bindC_wrespectful:
-    wrespectful7 (@_hpsim false) hpsim_bindC.
+    wrespectful8 (@_hpsim false) hpsim_bindC.
   Proof.
     econs; eauto using hpsim_bindC_mon; i.
     destruct PR. apply GF in SIM.
@@ -536,13 +672,13 @@ Section HPSIM.
       eapply _hpsim_mon_progress; eauto; clarify.
     - econs; eauto. rewrite <-!bind_bind. eapply IHSIM; eauto.
     - econs; eauto. rewrite <-!bind_bind. eapply IHSIM; eauto.
-    - econs; eauto. eauto 10 using rclo7, hpsim_bindC.
+    - econs; eauto. eauto 10 using rclo8, hpsim_bindC.
   Qed.
 
   Lemma hpsim_bindC_spec:
-    hpsim_bindC <8= gupaco7 (@_hpsim false) (cpn7 (@_hpsim false)).
+    hpsim_bindC <9= gupaco8 (@_hpsim false) (cpn8 (@_hpsim false)).
   Proof.
-    intros. eapply wrespect7_uclo; eauto with paco.
+    intros. eapply wrespect8_uclo; eauto with paco.
     apply hpsim_bindC_wrespectful.
   Qed.
 
@@ -551,23 +687,23 @@ Section HPSIM.
   
 
 
-  Variant hpsim_extendC (r: forall R (RR: Any.t * R -> Any.t * R -> iProp), bool -> bool -> Any.t * itree hAGEs R -> Any.t * itree hAGEs R -> Σ -> Prop):
-    forall R (RR: Any.t * R -> Any.t * R -> iProp), bool -> bool -> Any.t * itree hAGEs R -> Any.t * itree hAGEs R -> Σ -> Prop
+  Variant hpsim_extendC (r: forall R (RR: Any.t * R -> Any.t * R -> Σ -> iProp), bool -> bool -> Any.t * itree hAGEs R -> Any.t * itree hAGEs R -> Σ -> Σ -> Prop):
+    forall R (RR: Any.t * R -> Any.t * R -> Σ -> iProp), bool -> bool -> Any.t * itree hAGEs R -> Any.t * itree hAGEs R -> Σ -> Σ -> Prop
   :=
   | hpsim_extendC_intro
-      ps pt R RR sti_src sti_tgt fmr fmr'
-      (SIM: r R RR ps pt sti_src sti_tgt fmr)
+      ps pt R RR sti_src sti_tgt ctx fmr fmr'
+      (SIM: r R RR ps pt sti_src sti_tgt ctx fmr)
       (EXT: URA.extends fmr fmr')
-      (* (WF: URA.wf fmr') *)
-    :
-    hpsim_extendC r R RR ps pt sti_src sti_tgt fmr'
+      (WF: URA.wf fmr')
+     :
+    hpsim_extendC r R RR ps pt sti_src sti_tgt ctx fmr'
   .
 
   Lemma hpsim_extendC_mon
         r1 r2
-        (LEr: r1 <7= r2)
+        (LEr: r1 <8= r2)
     :
-    hpsim_extendC r1 <7= hpsim_extendC r2
+    hpsim_extendC r1 <8= hpsim_extendC r2
   .
   Proof. ii. destruct PR; econs; et. Qed.
 
@@ -576,22 +712,17 @@ Section HPSIM.
   Proof. reflexivity. Qed.
   
   Lemma hpsim_extendC_compatible:
-    compatible7 (@_hpsim false) hpsim_extendC.
+    compatible8 (@_hpsim false) hpsim_extendC.
   Proof.
     econs; eauto using hpsim_extendC_mon.
     intros. destruct PR. move SIM before RR. revert_until SIM.
-    induction SIM; econs; eauto using hpsim_extendC, URA_extends_refl; try (by 
-      iIntros "H"; iPoseProof (Own_extends EXT with "H") as "H"; iStopProof; eauto).
-    - i; eapply H; eauto using URA_extends_refl.
-      iIntros "H". iPoseProof (NEW with "H") as "H". iMod "H" as "[IP H]".
-      iFrame. iPoseProof (Own_extends EXT with "H") as "H". iStopProof. eauto.
-    - i; eapply H; eauto using URA_extends_refl.
-      iIntros "H". iPoseProof (NEW with "H") as "H". iMod "H" as "[IP H]".
-      iFrame. iPoseProof (Own_extends EXT with "H") as "H". iStopProof. eauto.
+    induction SIM; econs; eauto using hpsim_extendC, URA_extends_refl;
+      try (by etrans; cycle 1; eauto using Own_extends);
+      try (by i; eapply H; eauto; try refl; eapply URA.wf_mon in WF0; eauto).
   Qed.
 
   Lemma hpsim_extendC_spec:
-    hpsim_extendC <8= gupaco7 (@_hpsim false) (cpn7 (@_hpsim false)).
+    hpsim_extendC <9= gupaco8 (@_hpsim false) (cpn8 (@_hpsim false)).
   Proof.
     intros. gclo. econs; eauto using hpsim_extendC_compatible.
     eapply hpsim_extendC_mon, PR; eauto with paco.
@@ -645,21 +776,21 @@ Section HPSIM.
   
   Lemma hpsim_dummyC_src_mon
         r1 r2
-        (LEr: r1 <7= r2)
+        (LEr: r1 <8= r2)
     :
-    hpsim_dummyC_src r1 <7= hpsim_dummyC_src r2
+    hpsim_dummyC_src r1 <8= hpsim_dummyC_src r2
   .
   Proof. i. destruct PR; econs; eauto. Qed.
 
   Lemma hpsim_dummyC_src_compatible with_dummy:
-    compatible7 (@_hpsim with_dummy) hpsim_dummyC_src.
+    compatible8 (@_hpsim with_dummy) hpsim_dummyC_src.
   Proof.
     econs; eauto using hpsim_dummyC_src_mon; i. depdes PR.
     remember (st_src, i_src) as sti_src.
     remember (st_tgt, i_tgt) as sti_tgt.
     move SIM before RR. revert_until SIM.
     induction SIM; i; depdes Heqsti_src Heqsti_tgt;
-      grind; eauto 7 with paco imodL; r in DUMMY; des.
+      grind; eauto 8 with paco imodL; r in DUMMY; des.
     - assert (CASE:= case_itrH _ i); des; subst; itree_clarify DUMMY.
       destruct DUMMY1; subst; rewrite <-x; econs; eauto with imodL.
     - assert (CASE:= case_itrH _ i); des; subst; itree_clarify DUMMY.
@@ -736,7 +867,7 @@ Section HPSIM.
   Qed.
 
   Lemma hpsim_dummyC_src_spec (with_dummy:bool) :
-    hpsim_dummyC_src <8= gupaco7 (@_hpsim with_dummy) (cpn7 (@_hpsim with_dummy)).
+    hpsim_dummyC_src <9= gupaco8 (@_hpsim with_dummy) (cpn8 (@_hpsim with_dummy)).
   Proof.
     intros. gclo. econs; eauto using hpsim_dummyC_src_compatible.
     eapply hpsim_dummyC_src_mon, PR; eauto with paco.
@@ -755,21 +886,21 @@ Section HPSIM.
   
   Lemma hpsim_dummyC_tgt_mon
         r1 r2
-        (LEr: r1 <7= r2)
+        (LEr: r1 <8= r2)
     :
-    hpsim_dummyC_tgt r1 <7= hpsim_dummyC_tgt r2
+    hpsim_dummyC_tgt r1 <8= hpsim_dummyC_tgt r2
   .
   Proof. i. destruct PR; econs; eauto. Qed.
 
   Lemma hpsim_dummyC_tgt_compatible with_dummy:
-    compatible7 (@_hpsim with_dummy) hpsim_dummyC_tgt.
+    compatible8 (@_hpsim with_dummy) hpsim_dummyC_tgt.
   Proof.
     econs; eauto using hpsim_dummyC_tgt_mon; i. depdes PR.
     remember (st_src, i_src) as sti_src.
     remember (st_tgt, i_tgt) as sti_tgt.
     move SIM before RR. revert_until SIM.
     induction SIM; i; depdes Heqsti_src Heqsti_tgt;
-      grind; eauto 7 with paco imodL; r in DUMMY; des.
+      grind; eauto 8 with paco imodL; r in DUMMY; des.
     - assert (CASE:= case_itrH _ i); des; subst; itree_clarify DUMMY.
       destruct DUMMY1; subst; rewrite <-x; econs; eauto; imodIntroL.
     - assert (CASE:= case_itrH _ i); des; subst; itree_clarify DUMMY.
@@ -850,14 +981,14 @@ Section HPSIM.
   Qed.
 
   Lemma hpsim_dummyC_tgt_spec (with_dummy:bool) :
-    hpsim_dummyC_tgt <8= gupaco7 (@_hpsim with_dummy) (cpn7 (@_hpsim with_dummy)).
+    hpsim_dummyC_tgt <9= gupaco8 (@_hpsim with_dummy) (cpn8 (@_hpsim with_dummy)).
   Proof.
     intros. gclo. econs; eauto using hpsim_dummyC_tgt_compatible.
     eapply hpsim_dummyC_tgt_mon, PR; eauto with paco.
   Qed.
   
   Lemma hpsim_le_gpaco with_dummy r r':
-    @hpsim <7= gpaco7 (@_hpsim with_dummy) (cpn7 (@_hpsim with_dummy)) r r'.
+    @hpsim <8= gpaco8 (@_hpsim with_dummy) (cpn8 (@_hpsim with_dummy)) r r'.
   Proof.
     gcofix CIH. i. punfold PR.
     induction PR; pclearbot; eauto with paco;
@@ -871,19 +1002,18 @@ Section HPSIM.
   Hint Resolve hpsim_le_gpaco: paco.
 
   Corollary hpsim_add_dummy:
-    @hpsim <7= paco7 (@_hpsim true) bot7.
+    @hpsim <8= paco8 (@_hpsim true) bot8.
   Proof. ginit. eauto with paco. Qed.
 *)
 
   Definition hpsim_fsem: relation (Any.t -> itree hAGEs Any.t) :=
-    (eq ==> (fun itr_src itr_tgt => forall st_src st_tgt (INV: Ist st_src st_tgt ε),
-                hpsim_body false false (st_src, itr_src) (st_tgt, itr_tgt) ε))%signature.
+    (eq ==> hpsim_fun)%signature.
 
   Definition hpsim_fnsem: relation (string * (Any.t -> itree hAGEs Any.t)) := RelProd eq hpsim_fsem.
 
   (* Arguments _hpsim {with_dummy} hpsim {R} RR.
 
-  Definition hpsim {R} RR := paco7 (@_hpsim false) bot7 R RR.
+  Definition hpsim {R} RR := paco8 (@_hpsim false) bot8 R RR.
 
   Definition hpsim_end : Any.t*Any.t -> Any.t*Any.t -> iProp :=
     fun '(st_src, v_src) '(st_tgt, v_tgt) => Ist st_src st_tgt ** ⌜v_src = v_tgt⌝. *)
@@ -891,62 +1021,28 @@ Section HPSIM.
 End HPSIM.
 
 Hint Resolve _hpsim_mon: paco.
-Hint Resolve cpn7_wcompat: paco.
+Hint Resolve cpn8_wcompat: paco.
 
 (**********)
 
-
 Lemma hpsim_refl {Σ: GRA.t}:
-  forall st itr fl fmr,
-    hpsim_body fl fl (fun src tgt => ⌜src = tgt⌝%I) false false (st, itr) (st, itr) fmr.
+  forall st itr fl ctx fmr (WF: URA.wf (fmr ⋅ ctx)),
+  hpsim_body fl fl (fun src tgt => ⌜src = tgt⌝%I) false false (st, itr) (st, itr) ctx fmr.
 Proof.
-  ginit. gcofix CIH. i. ides itr.
-  { gstep. eapply hpsim_ret; ss.
-    iIntros "H". et.
-  }
-  { guclo hpsimC_spec. econs. 
-    guclo hpsimC_spec. econs. 
-    eapply hpsim_progress_flag. gbase. auto.
-  }
-  destruct e.
-  { dependent destruction h; rewrite <-! bind_trigger; resub.
-    - guclo hpsimC_spec. econs. { instantiate (1:= ⌜True⌝%I). et. }
-      guclo hpsimC_spec. econs; et.
-      ii. eapply hpsim_progress_flag. gbase. et.
-    - guclo hpsimC_spec. econs 17. { instantiate (1:= ⌜True⌝%I). et. }
-      guclo hpsimC_spec. econs; et.
-      ii. eapply hpsim_progress_flag. gbase. et.
-  }
-  destruct e.
-  { dependent destruction c. rewrite <- ! bind_trigger. resub.
-    gstep.
-    eapply hpsim_call; ss. { instantiate (1:= ⌜True⌝%I). et. }
-    ii. econs; et.
-    exploit (@own_pure _ (st_src0 = st_tgt0) _ WF).
-    { iIntros "H". iPoseProof (INV with "H") as "H".
-      iApply Upd_Pure. iDestruct "H" as "[H _]". eauto. }
-    i. subst. gbase. eauto.
-  }
-  destruct s.
-  { rewrite <- ! bind_trigger. resub. dependent destruction s.
-    destruct (run st) eqn:RUN.
-    guclo hpsimC_spec. econs; et. 
-    guclo hpsimC_spec. econs; et. 
-    eapply hpsim_progress_flag. gbase. et.
-  }
-  { rewrite <- ! bind_trigger. resub. dependent destruction e.
-    { guclo hpsimC_spec. econs 9. i.
-      guclo hpsimC_spec. econs.
-      eapply hpsim_progress_flag. gbase. eauto.
-    }
-    { guclo hpsimC_spec. econs 10. i.
-      guclo hpsimC_spec. econs.
-      eapply hpsim_progress_flag. gbase. eauto.
-    }
-    { guclo hpsimC_spec. econs. i.
-      eapply hpsim_progress_flag. gbase. eauto.
-    }
-  }
+  ginit. gcofix CIH. i.
+  gstep. assert (CASE := case_itrH _ itr); des; subst.
+  - econs; eauto.
+  - repeat (econs; eauto with paco).
+  - repeat (econs; eauto with paco).
+  - repeat (econs; eauto with paco).
+  - destruct c; econs; eauto.
+    { instantiate (1:= Own fmr). iIntros "H". iSplitR; eauto. }
+    i. uipropall. edestruct INV; rr; eauto. des.
+    rr in H0. uipropall. subst.
+    repeat (econs; eauto with paco).
+  - destruct s. destruct (run st) eqn:RUN.
+    repeat (econs; eauto with paco).
+  - depdes e; repeat (econs; eauto with paco).
 Qed.
 
 
@@ -961,13 +1057,12 @@ Section HPSIMMODSEM.
   Definition fl_src := ms_src.(HModSem.fnsems).
   Definition fl_tgt := ms_tgt.(HModSem.fnsems).
 
-  Let W: Type := (Any.t) * (Any.t).
   Inductive sim: Prop := mk {
     Ist: Any.t -> Any.t -> iProp;
     hpsim_fnsems: Forall2 (hpsim_fnsem fl_src fl_tgt Ist) ms_src.(HModSem.fnsems) ms_tgt.(HModSem.fnsems);
-    hpsim_initial: Ist (ms_src.(HModSem.initial_st)) (ms_tgt.(HModSem.initial_st)) ε;
-    (* sim_fnsems: Forall2 (sim_fnsem wf le fl_src fl_tgt) ms_src.(ModSem.fnsems) ms_tgt.(ModSem.fnsems); *)
-    (* sim_initial: exists w_init, wf w_init (ms_src.(HModSem.initial_st), ms_tgt.(HModSem.initial_st)); *)
+
+    (* TODO: Fix the following wrong design. *)
+    hpsim_initial: Own ε ⊢ Ist (ms_src.(HModSem.initial_st)) (ms_tgt.(HModSem.initial_st));
   }.
 
 End HPSIMMODSEM.
@@ -976,13 +1071,14 @@ Lemma self_sim {Σ: GRA.t} (ms: HModSem.t):
   sim ms ms.
 Proof.
   econs; et.
-  - instantiate (1:=(fun src tgt => ⌜src = tgt⌝%I)). (* fun p => fst p = snd p *)
+  - instantiate (1:=(fun src tgt => ⌜src = tgt⌝%I)).
     generalize (HModSem.fnsems ms).
     induction a; ii; ss.
     econs; et. econs; ss. ii; clarify.
-    rr in INV. uipropall. clarify.
-    eapply hpsim_refl.
-  - rr. uipropall.
+    eapply own_pure in INV; eauto; cycle 1.
+    { eapply URA.wf_mon. eauto. }
+    subst. eapply hpsim_refl; eauto.
+  - iIntros "H". eauto.
 Qed.
 
 End HModSemPair.
